induction suggested  by Henrik

GateOptimization/Basic.lean
@@ -10,9 +10,75 @@ def and_gate (x y : Bool) : Bool :=
 
 inductive Net where
 | term: Bool -> Net
+--| input: String -> Net
 | and: Net -> Net -> Net
 | or: Net -> Net -> Net
+deriving Repr
 
--- derive Repr
+def f: Net := Net.term false
+def t: Net := Net.term true
+def i (b:Bool) : Net := Net.term b
 
-def n: Net := Net.term false
+
+
+def net_eval (n:Net) : Bool :=
+  match n with
+  | Net.term b => b
+  | Net.and x y => (net_eval x) && (net_eval y)
+  | Net.or x y =>  (net_eval x) || (net_eval y)
+
+
+#eval net_eval t
+#eval net_eval f
+
+#eval net_eval (.and t f)
+#eval net_eval (.and t t)
+
+def net_min (n:Net) : Net :=
+  match n with
+  | .term _              => n
+  | .and l r =>
+    match net_min l, net_min r with
+    | .term false, _
+    | _, .term false     => .term false
+    | ll, rr             => .and ll rr
+  | .or l r =>
+    match net_min l, net_min r with
+    | .term true, _
+    | _, .term true     => .term true
+    | ll, rr             => .or ll rr
+
+#eval net_min (.and t t)
+#eval net_min (.and (.and f t) t)
+#eval net_min (.and (.or t f) t)
+#eval net_min (.or t (.or t f))
+
+theorem net_min_correct : ∀ n, net_eval n = net_eval (net_min n) := by
+  intro n
+  induction n using net_min.induct <;> simp [net_eval, net_min, *]
+
+-- theorem net_min_proof:  ∀ n, net_eval (net_min n) = net_eval n := by
+--   intro n
+--   induction n
+--   . simp [net_min, net_eval]
+--   . rw [net_min]
+--     split
+--     .
+--     . sorry
+--     sorry
+--   . sorry
+
+
+
+  -- rw [net_min.eq_def]
+  -- cases n
+  -- . simp
+  -- .
+  -- . sorry
+
+
+
+  -- cases (net_min n)
+  -- .
+  -- . sorry
+  -- . sorry
